proof/DDC/Language/SystemF2Store/Progress.v
@@ -1,0 +1,181 @@
+
+Require Import DDC.Language.SystemF2Store.Step.
+Require Import DDC.Language.SystemF2Store.TyJudge.
+Require Import DDC.Language.SystemF2Store.Exp.
+Require Import DDC.Base.
+
+
+(* If we have a well typed case match on a store location containing some 
+   data object, then there is a case alternative corresponding to
+   that object's data constructor. *)
+Lemma getAlt_has
+ :  forall ds se ss l dc svs alts t
+ ,  WfS ds se ss
+ -> get l ss = Some (SObj dc svs)
+ -> TYPE ds nil nil se (XCase (XLoc l) alts) t
+ -> (exists x, getAlt dc alts = Some (AAlt dc x)).
+Proof.
+ intros.
+ eapply getAlt_exists.
+ inverts_type.
+ nforall. 
+ assert (In dc dcs).
+  rewrite H6 in H3. inverts H3.
+  have (getCtorOfType (TCon tc) = Some tc) as HC.
+  inverts H. int.
+  unfold STORET in H4.
+   spec H4 H0.
+   dest tcObj. dest tsParam. dest tsFields.
+   int.
+   rewrite H4 in H2. inverts H2.
+   erewrite getCtorOfType_makeTApps with (tc := tcObj) in H6; eauto.
+    inverts H6.
+   eauto.
+ eauto.
+Qed.
+Hint Resolve getAlt_has.
+
+
+
+(* A well typed expression is either a well formed value, 
+   or can transition to the next state. *)
+Theorem progress
+ :  forall ds x t
+ ,  DEFSOK ds
+ -> TYPE ds nil nil x t
+ -> value x \/ (exists x', STEP x x').
+Proof.
+ intros. gen t.
+ induction x using exp_mutind with 
+  (PA := fun a => a = a)
+  ; intros.
+
+
+ Case "XVar".
+  nope.
+
+
+ Case "XLAM".
+  left. apply type_wfX in H0. auto.
+
+
+ Case "XAPP".
+  inverts keep H0.
+  edestruct IHx. eauto.
+  SCase "x value".
+   right. inverts H1. inverts H3.
+    SSCase "x = XVar". nope.
+    SSCase "x = XLAM". exists (substTX 0 t2 x1). eapply EsLAMAPP.
+    SSCase "x = XAPP". nope.
+    SSCase "x = XApp". nope.
+    SSCase "x = XCon".
+     inverts_type.
+     have (takeTCon (TCon tc0) = takeTCon (TForall t0)). nope.
+    SSCase "x = XCase".
+     nope.
+  SCase "x steps".
+   right.
+    dest x'.
+    exists (XAPP x' t2).
+    lets D: EsContext XcAPP H1.
+    eauto.
+
+
+ Case "XLam".
+  left. eapply type_wfX in H0. auto.
+
+
+ Case "XApp".
+  right.
+  inverts_type.
+  edestruct IHx1; eauto.
+  SCase "value x1".
+   edestruct IHx2; eauto.
+    SSCase "value x2".
+     have (exists t x, x1 = XLam t x) as HF.
+     destruct HF as [t11].
+     destruct H2 as [x12].
+     subst.
+     exists (substXX 0 x2 x12). 
+     apply EsLamApp; eauto.
+    SSCase "x2 steps".
+     destruct H1 as [x2'].
+     exists (XApp x1 x2'). auto.
+  SCase "x1 steps".
+   destruct H0  as [x1'].
+   exists (XApp x1' x2).
+   eapply (EsContext (fun xx => XApp xx x2)); auto.
+
+
+ Case "XCon".
+  inverts_type.
+  (* All ctor args are either wnf or can step *)
+  assert (Forall (fun x => wnfX x \/ (exists x', STEP x x')) xs) as HWS.
+   nforall. intros.
+   have (exists t, TYPE ds nil nil x t). dest t.
+   have (value x \/ (exists x', STEP x x')). int.     
+
+  (* All ctor args are wnf, or there is a context where one can step *)
+  lets D: (@exps_ctx_run exp exp) HWS.
+  inverts D.
+   (* All ctor args are wnf *)
+   left.
+   assert (Forall (wfT 0) ts).
+    rrwrite (0 = length (@nil ki)).
+    eapply kind_wfT_Forall2. eauto.
+
+   assert (Forall (wfX 0 0) xs).
+    have    (0 = length (@nil ki)) as HKL. rewrite HKL at 1.
+    rrwrite (0 = length (@nil ty)). eauto.
+   eauto.
+
+   (* There is a context where one ctor arg can step *)
+   right.
+    dest C. dest x'.
+    int. subst.
+    lets D: step_context_XCon_exists H2 H4.
+    destruct D as [x'']. eauto.
+
+
+ Case "XCase".
+  right.
+  inverts keep H1.
+  have (value x \/ (exists x', STEP x x')) as HS.
+  inverts HS. clear IHx.
+
+  (* Discriminant is a value *)
+  SCase "x value".
+   destruct x; nope.
+
+    (* Can't happen, 
+       TForall has no data type constructor *)
+    SSCase "XCase (XLAM x) aa".
+     have (exists t', tObj = TForall t').
+     dest t'. subst. false.
+
+    (* Can't happen, 
+       tFun has no data type constructor *)
+    SSCase "XCase (XLam t x) aa".
+     have (exists t11 t12, tObj = tFun t11 t12).
+     dest t11. dest t12. subst.
+     unfold tFun in H6. simpl in H6. inverts H6.
+     have (DEFOK ds (DefDataType TyConFun ks dcs)) as HD.
+     inverts HD. false.
+
+    (* When we have a well typed case match on some data object, 
+       then there is a corresponding alternative. *)
+    SSCase "XCon".
+     have (exists x, getAlt d aa = Some (AAlt d x)).
+     dest x. exists (substXXs 0 l0 x).
+     eapply EsCaseAlt; eauto.
+
+  (* Discriminant steps *)
+  SCase "x steps".
+   destruct H2 as [x'].
+   exists (XCase x' aa).
+   lets D: EsContext XcCase; eauto.
+
+ Case "XAlt".
+   auto.     
+Qed.
+
